\documentclass[a4paper]{article}

\usepackage[left=1cm,right=1cm,top=1.5cm,bottom=1.5cm]{geometry}
\usepackage{amsmath}
\usepackage{amssymb}
\usepackage{multicol}


\begin{document}

\begin{multicols}{2}

\section*{Discrete Pair of RVs}

\subsection*{Joint CDF}

\noindent $F_{X, Y}(x, y) = P[X \le x, Y \le y]$ \\
\vspace{10px}
\noindent $0 \le F_{X, Y}(x, y) \le 1$ \\
\vspace{10px}
\noindent $F_{X}(x) = F_{X, Y}(x, \infty) \rightarrow \textbf{ Marginal CDF of } X$ \\
\vspace{10px}
\noindent $F_{Y}(y) = F_{X, Y}(\infty, y) \rightarrow \textbf{ Marginal CDF of } Y$ \\
\vspace{10px}
\noindent $F_{X, Y}(x, -\infty) = F_{X, Y}(-\infty, y) = 0$ \\
\vspace{10px}
\noindent $x_{1} \le x_{2} \textbf{and} y_{1} \le y_{2} \rightarrow F_{X, Y}(x_{1}, y_{1}) \le F_{X, Y}(x_{2}, x_{2})$ \\
\vspace{10px}
\noindent $F_{X, Y}(\infty, \infty) = 1$ \\
\vspace{10px}

\subsection*{Joint PMF}

$P_{X, Y}(x, y) = P[X = x, Y = y]$ \\

$\displaystyle\sum_{x} \displaystyle\sum_{y} P_{X ,Y}(x, y) = 1$ \\


\subsection*{Marginal PMF}

$P_{Y}(y) = \displaystyle\sum_{x} P_{X, Y}(x, y)$ \\
\vspace{10px}
$P_{X}(x) = \displaystyle\sum_{y} P_{X, Y}(x, y)$ \\

\columnbreak

\section*{Continuous Pair of RVs}

\subsection*{Joint CDF}

\noindent $F_{X, Y}(x, y) = \displaystyle\int_{-\infty}^{x} \displaystyle\int_{-\infty}^{y} f_{X, Y}(u, v) d u d v$ \\
\vspace{10px}

\begin{flalign*}
    P[x_{1} < X \le x_{2}, y_{1} < Y \le y_{2}] & = F_{X, Y}(x_{1}, y_{1}) - F_{X, Y}(x_{1}, y_{2}) && \\
    &- F_{X, Y}(x_{2}, y_{1}) + F_{X, Y}(x_{2}, y_{2}) && \\
\end{flalign*}

\subsection*{Joint PDF}

\noindent $f_{X, Y}(x, y) = \frac{\partial^{2} F_{X, Y}(x, y)}{\partial x \partial y}$
\vspace{10px}
\noindent $P_{X, Y}(x, y) = P[X = x, Y = y]$ \\
\vspace{10px}
\noindent $P[x < X \le x + d x, y < Y \le y + d y] = f_{X, Y}(x, y) d x d y$ \\
\vspace{10px}
\noindent $f_{X, Y}(x, y) \ge 0, \forall{(x, y)}$
\vspace{10px}
\noindent $\displaystyle\int_{-\infty}^{\infty}\displaystyle\int_{-\infty}^{\infty}f_{X ,Y}(x, y) d x d y= 1$ \\

\subsection*{Marginal PDF}

$f_{X}(x) = \displaystyle\int_{-\infty}^{\infty} f_{X, Y}(x, y) d y$ \\

\noindent $f_{Y}(y) = \displaystyle\int_{-\infty}^{\infty} f_{X, Y}(x, y) d x$ \\

\section*{Integration with Polar Coordination}

$x = r \cos{\theta}$ and $y = r \sin{\theta}$

\noindent Then substitute and do it as normal \\

\end{multicols}

\thispagestyle{empty}
\end{document}
